

Assignment 4

Name:- Muhammad Asham Azam

Roll# L1S22BSCSO413

Section:- E7

Q1a) i) t^2

Solution:-

$$\mathcal{L}\{f(t)\} = \int_0^{\infty} e^{-st} f(t) dt$$

$$\mathcal{L}\{t^2\} = \int_0^{\infty} e^{-st} t^2 dt$$

Integration using DI method.

+	0	$\xrightarrow{\quad}$	\bar{I}
-	t^2	\searrow	e^{-st}
+	$2t$	\searrow	$-e^{-st}/s$
-	2	\searrow	e^{-st}/s^2
+	0	\searrow	$-e^{-st}/s^3$

$$= \lim_{b \rightarrow \infty} \left[-\frac{t^2 e^{-st}}{s} - \frac{2te^{-st}}{s^2} - \frac{2e^{-st}}{s^3} \right]_0^b$$

$$= \left(-\frac{b^2 e^{-sb}}{s} - \frac{2be^{-sb}}{s^2} - \frac{2e^{-sb}}{s^3} \right) - \left(-0 - 0 - \frac{2}{s^3} \right)$$

$$\text{as } b \rightarrow \infty, e^{-sb} \rightarrow 0$$

$$= 0 + \frac{2}{s^3}$$

$$= \frac{2}{s^3}$$

ii) e^{-st}

Solution

$$\mathcal{L}\{e^{-st}\} = \int_0^{\infty} e^{-st} e^{-st} dt$$

$$= \int_0^{\infty} e^{t(-s-s)} dt$$

$$= \lim_{b \rightarrow \infty} \left. \frac{e^{t(-s-s)}}{-s-s} \right|_0^b$$

$$= \frac{e^{b(-s-s)}}{-s-s} - \frac{1}{-s-s}$$

$$= 0 - \frac{1}{-s-s} = \frac{1}{s+s}$$

iii) $\sinh 3t$

Solution

$$\mathcal{L}\{\sinh 3t\} = \int_0^{\infty} st e^{-st} \sinh 3t dt$$

Integration by parts using DI method.

	D	I
+	$\sinh 3t$	e^{-st}
-	$3 \cosh 3t$	$-e^{-st}/s$
+	$9 \sinh 3t$	e^{-st}/s^2

$$= \lim_{b \rightarrow \infty} \left. -\frac{e^{-st}}{s} \sinh 3t - \frac{e^{-st}}{s^2} 3 \cosh 3t \right|_0^b + \frac{9}{s^2} \int_0^{\infty} e^{-st} \sinh 3t dt$$

$$= 0 - \left(\frac{-\sinh 0}{s} - \frac{3 \cosh 0}{s^2} \right) + \frac{9}{s^2} \mathcal{L}\{\sinh 3t\}$$

$$= 0 + \frac{3}{s^2} + \frac{9}{s^2} \mathcal{L}\{\sinh 3t\}$$

$$\mathcal{L}\{\sinh 3t\} = \frac{3}{s^2} + \frac{9}{s^2} \mathcal{L}\{\sinh 3t\}$$

$$\mathcal{L}\{\sinh 3t\} - \frac{9}{s^2} \mathcal{L}\{\sinh 3t\} = \frac{3}{s^2}$$

$$s^2 \mathcal{L}\{\sinh 3t\} - 9 \mathcal{L}\{\sinh 3t\} = 3$$

$$\mathcal{L}\{\sinh 3t\} (s^2 - 9) = 3$$

$$\mathcal{L}\{\sinh 3t\} = \frac{3}{s^2 - 9}$$

Q1)b)

i) $\sin(5t+2)$

solution

$$\sin(\alpha + \beta) = \sin \alpha \cos \beta + \cos \alpha \sin \beta$$

$$\sin(5t+2) = \sin 5t \cos 2 + \cos 5t \sin 2$$

$$\mathcal{L}\{\sin(5t+2)\} = \mathcal{L}\{\sin 5t \cos 2\} + \mathcal{L}\{\cos 5t \sin 2\}$$

$$= \cos 2 \mathcal{L}\{\sin 5t\} + \sin 2 \mathcal{L}\{\cos 5t\}$$

$$= \cos 2 \left(\frac{5}{s^2 + 25} \right) + \sin 2 \left(\frac{s}{s^2 + 25} \right)$$

$$= \frac{s \sin 2 + s \cos 2}{s^2 + 2s}$$

ii) ~~e^{-st}~~
solution

~~$$\mathcal{L}\{e^{at}\} = \frac{1}{s-a}$$~~

~~$$\mathcal{L}\{e^{-st}\} = \frac{1}{s+s}$$~~

iii) $t \sin t$
solution

$$\mathcal{L}\{t f(t)\} = -\frac{d}{ds} (\mathcal{L}\{f(t)\})$$

$$\mathcal{L}\{t \sin t\} = -\frac{d}{ds} \left(\frac{1}{s^2+1} \right)$$

$$= - \left(\frac{0 - 2s}{(s^2+1)^2} \right)$$

$$= \frac{2s}{(s^2+1)^2}$$

ii) $e^{-t} \sin 2t$

Solution:- $\mathcal{L}\{e^{at} f(t)\} = F(s-a)$

$\mathcal{L}\{e^{-t} \sin 2t\} = F(s+1)$

$F(s) = \mathcal{L}\{\sin 2t\} = \frac{2}{s^2+4}$

$F(s+1) = \frac{2}{s^2+4} + 1$

$= \frac{2+s^2+4}{s^2+4} = \frac{s^2+6}{s^2+4}$

$F(s+1) = \frac{2}{(s+1)^2+4}$

Q1)c)

i) $\frac{s-2}{s^2+3}$

Solution

$\frac{s-2}{s^2+3} = \frac{s}{s^2+3} - \frac{2}{s^2+3}$

$\mathcal{L}^{-1}\left\{\frac{s-2}{s^2+3}\right\} = \mathcal{L}^{-1}\left\{\frac{s}{s^2+3} - \frac{2}{s^2+3}\right\}$

$= \mathcal{L}^{-1}\left\{\frac{s}{s^2+(\sqrt{3})^2}\right\} - \frac{2}{\sqrt{3}} \mathcal{L}^{-1}\left\{\frac{\sqrt{3}}{s^2+(\sqrt{3})^2}\right\}$

$$= \cos \sqrt{3}t - \frac{2}{\sqrt{3}} \sin \sqrt{3}t$$

ii) $\frac{3}{s(s^2+4)}$

Solution -

$$\mathcal{L}^{-1} \left\{ \frac{3}{s(s^2+4)} \right\} = 3 \mathcal{L}^{-1} \left\{ \frac{1}{s(s^2+4)} \right\}$$

$$= 3 \mathcal{L}^{-1} \left\{ \frac{1/4}{s} - \frac{s}{4(s^2+2^2)} \right\}$$

$$= 3 \mathcal{L}^{-1} \left\{ \frac{1/4}{s} - \left(\frac{1}{4} \right) \left(\frac{s}{s^2+2^2} \right) \right\}$$

$$= 3 \left(\frac{1}{4} \mathcal{L}^{-1} \left\{ \frac{1}{s} \right\} - \frac{1}{4} \mathcal{L}^{-1} \left\{ \frac{s}{s^2+2^2} \right\} \right)$$

$$= 3 \left(\frac{1}{4} (1) - \frac{1}{4} \cos 2t \right)$$

$$= \frac{3}{4} - \frac{3 \cos 2t}{4}$$

Q1) d)

$$i) y'' + 2y' + 5y = 0$$

$$y(0) = 1$$

$$y'(0) = 1$$

solution:-

$$y'' + 2y' + 5y = 0$$

Taking Laplace Transform on b.s

$$\mathcal{L}\{y''\} + 2\mathcal{L}\{y'\} + 5\mathcal{L}\{y\} = 0$$

$$s^2 Y(s) - sy(0) - y'(0) + 2[sY(s) - y(0)] + 5Y(s) = 0$$

$$s^2 Y(s) - s - 1 + 2sY(s) - 2 + 5Y(s) = 0$$

$$Y(s)(s^2 + 2s + 5) = s + 3$$

$$Y(s) = \frac{s+3}{s^2+2s+5}$$

$$Y(s) = \frac{s+1}{s^2+2s+1+4} + 2$$

$$Y(s) = \frac{s+1}{(s+1)^2+2^2} + \frac{2}{(s+1)^2+2^2}$$

Taking inverse Laplace

$$\mathcal{L}^{-1}(Y(s)) = \mathcal{L}^{-1}\left(\frac{s+1}{(s+1)^2+2^2}\right) + \mathcal{L}^{-1}\left(\frac{2}{(s+1)^2+2^2}\right)$$

$$y(t) = \mathcal{L}^{-1}\{F_1(s+1)\} + \mathcal{L}^{-1}\{F_2(s+1)\}$$

$$F_1(s) = \mathcal{L}\{\cos 2t\}$$

$$F_2(s) = \mathcal{L}\{\sin 2t\}$$

we know

$$\mathcal{L}\{e^{at} f(t)\} = F(s-a), \text{ where } F(s) = \mathcal{L}\{f(t)\}$$

So,

$$y(t) = e^{-t} \cos 2t + e^{-t} \sin 2t.$$

$$\text{ii) } y'' + 9y = 3 \sin 3t$$

$$y(0) = 1$$

$$y'(0) = 0$$

solution

$$\mathcal{L}\{y''\} + 9\mathcal{L}\{y\} = \mathcal{L}\{3 \sin 3t\}$$

$$s^2 Y(s) - sy(0) - y'(0) + 9(Y(s)) = \frac{3}{s^2 + 9}$$

$$Y(s)(s^2 + 9) - s - 0 = \frac{3}{s^2 + 9}$$

$$Y(s) = \frac{3}{(s^2 + 9)^2} + \frac{s}{s^2 + 9}$$

Taking inverse Laplace Transform.

$$\mathcal{L}^{-1}\{Y(s)\} = \mathcal{L}^{-1}\left\{\frac{3}{(s^2 + 9)^2}\right\} + \mathcal{L}^{-1}\left\{\frac{s}{s^2 + 9}\right\}$$

$$= \mathcal{L}^{-1}\left\{\frac{1}{18} \cdot \frac{2 \cdot 3^3}{(s^2 + 9)^2}\right\} + \mathcal{L}^{-1}\left\{\frac{s}{s^2 + 3^2}\right\}$$

$$= \frac{1}{18} \mathcal{L}^{-1}\left\{\frac{2 \cdot 3^3}{(s^2 + 3^2)^2}\right\} + \mathcal{L}^{-1}\left\{\frac{s}{s^2 + 3^2}\right\}$$

We know,

$$\mathcal{L}^{-1} \left\{ \frac{2a^3}{(s^2 + a^2)^2} \right\} = \sin at - at \cos at$$

$$y(t) = \frac{1}{18} (\sin 3t - 3t \cos 3t) + \sin 2t \cos 3t$$

$$\text{Q2) } 2y''' + 3y'' - 3y' - 2y = e^{-t}$$

$$y(0) = 0$$

$$y'(0) = 0$$

$$y''(1) = 2$$

solution

The problem is $y''(1) = 2$, it should be $y'(0) = 2$

So,

$$2\mathcal{L}\{y'''\} + 3\mathcal{L}\{y''\} - 3\mathcal{L}\{y'\} - 2\mathcal{L}\{y\} = \mathcal{L}\{e^{-t}\}$$

$$2[s^3 Y(s) - s^2 y(0) - s y'(0) - y''(0)] + 3[s^2 Y(s) - s y'(0) - y''(0)] - 3[s Y(s) - y(0)] - 2[Y(s)] = \frac{1}{s+1}$$

$$Y(s)(2s^3 + 3s^2 - 3s - 2) - 4 = \frac{1}{s+1}$$

$$Y(s)(2s^3 + 3s^2 - 3s - 2) = \frac{4s+5}{s+1}$$

$$Y(s) = \frac{4s+5}{(s+1)(2s^3 + 3s^2 - 3s - 2)}$$

$$\begin{array}{r|rrrr} 1 & 2 & 3 & -3 & -2 \\ & & 2 & 5 & 2 \\ \hline & 2 & 5 & 2 & 0 \end{array}$$

$$Y(s) = \frac{4s+5}{(s+1)(s-1)(2s^2+5s+2)}$$

$$Y(s) = \frac{4s+5}{(s+1)(s-1)(s+2)(2s+1)}$$

$$\frac{4s+5}{(s+1)(s-1)(s+2)(2s+1)} = \frac{A}{s+1} + \frac{B}{s-1} + \frac{C}{s+2} + \frac{D}{2s+1}$$

$$4s+5 = \frac{A(s-1)(s+2)(2s+1)}{(2s+1)} + \frac{B(s+1)(s+2)(2s+1)}{(2s+1)} + \frac{C(s-1)(s+1)}{(s+2)} + \frac{D(s-1)(s+1)(s+2)}{(2s+1)}$$

$$s = 1$$

$$9 = B(2)(3)(3)$$

$$B = \frac{9}{18} = \frac{1}{2}$$

$$s = -1$$

$$1 = A(-2)(1)(-1)$$

$$A = \frac{1}{2}$$

$$s = -2$$

$$-3 = C(-3)(-1)(-3)$$

$$C = \frac{1}{3}$$

$$s = -\frac{1}{2}$$

$$3 = 0\left(\frac{1}{2}\right)\left(-\frac{3}{2}\right)\left(-\frac{3}{2}\right)$$

$$D = \frac{8}{3}$$

$$\mathcal{L}^{-1}\{Y(s)\} = \frac{1}{3} \mathcal{L}^{-1}\left\{\frac{1}{s+1}\right\} + \frac{1}{2} \mathcal{L}^{-1}\left\{\frac{1}{s-1}\right\} + \frac{1}{3} \mathcal{L}^{-1}\left\{\frac{1}{s+2}\right\} + \frac{8}{3} \mathcal{L}^{-1}\left\{\frac{1}{2s+1}\right\}$$

$$y(t) = \frac{1}{2} e^{-t} + \frac{1}{2} e^t + \frac{1}{3} e^{-2t} + \frac{4}{3} e^{-t/2}$$

Q3)

$$y'' - xy = \sin x$$

Solution

$$y'' - xy = \sin x$$

$$y(x) = \sum_{n=0}^{\infty} a_n x^n$$

$$y'(x) = \sum_{n=1}^{\infty} n a_n x^{n-1}$$

$$y''(x) = \sum_{n=2}^{\infty} n(n-1) a_n x^{n-2}$$

$$m = n-2$$

$$\sum_{m=0}^{\infty} (m+2)(m+1)a_{m+2} x^m$$

$$k = n+1$$

$$\sum_{k=1}^{\infty} a_{k-1} x^k$$

$$\sum_{m=0}^{\infty} (m+2)(m+1)a_{m+2} x^m - \sum_{k=1}^{\infty} x^k = \sin(x)$$

$$(0+2)(0+1)a_2 + \sum_{m=1}^{\infty} (m+2)(m+1)a_{m+2} x^m = \sin x$$

$$\sin(x) = x - \frac{x^3}{6} + \frac{x^5}{120}$$

$$x^0 = 2a_2 = 0$$

$$x^1 = 6a_3 - a_0 = 1$$

$$x^2 = 12a_4 - a_2 = \frac{1}{6}$$

$$x^3 = 20a_5 - a_3 = -\frac{1}{6}$$

$$a_2 = 0$$

$$a_3 = \frac{1}{6} a_0$$

$$a_4 = \frac{1}{12} a_2$$

$$a_5 = -\frac{1}{120} a_3$$

$$y(x) = 1 + \frac{1}{6} x^3 + \frac{1}{12} x^4 + \dots$$

$$ii) y'' - xy = x^2$$

$$y(0) = 1$$

$$y'(0) = 0$$

Solution

$$= \sum_{n=2}^{\infty} n(n-1)a_n x^{n-2} - \sum_{n=0}^{\infty} a_n x^{n+1} = x^2$$

$$m = n - 2$$

$$\sum_{m=0}^{\infty} (m+2)(m+1)a_{m+2} x^m$$

$$\sum_{k=1}^{\infty} a_{k-1} x^k$$

$$\sum_{k=1}^{\infty} a_{k-1} x^k$$

$$\sum_{m=0}^{\infty} (m+2)(m+1)a_{m+2} x^m - \sum_{k=1}^{\infty} a_{k-1} x^k = x^2$$

$$x^0 = 2a_2 = 0$$

$$x^1 = 6a_3 - a_0 = 0$$

$$x^2 = 12a_4 - a_1 = 1$$

$$x^3 = 20a_5 - a_2 = 0$$

$$a_3 = \frac{1}{6}$$

$$a_4 = \frac{1}{12}$$

$$a_5 = 0$$

$$y(x) = 1 + \frac{1}{6} x^3 + \frac{1}{12} x^4$$